WIP

languages/decrement-builtin/run.ml
@@ -1,5 +1,10 @@
+open Core
+open Libminuskapluginbase
+open Pluginbase
+
 let main () =
   Libminuska.Miskeleton.main
+    (get_primitive_value_algebra (coqModuleName_of_sexp (Sexp.of_string ("(Std_module klike)"))))
     Internal.chosen_builtins
     Transform.parse
     Internal.lang_interpreter
