languages/imp/run.ml
@@ -1,8 +1,11 @@
 open Core
-open Printf
+open Libminuskapluginbase
+open Pluginbase
+
 
 let main () =
   Libminuska.Miskeleton.main
+    (get_primitive_value_algebra (coqModuleName_of_sexp (Sexp.of_string ("(Std_module klike)"))))
     Imp.Internal.chosen_builtins
     Imp.Transform.parse
     Imp.Internal.lang_interpreter
