coq-minuska/theories/frontend.v
@@ -4,6 +4,7 @@ From Minuska Require Import
     notations
     default_static_model
     builtins
+    properties
 .
 
 Arguments e_fun {Σ} f l%_list_scope.
@@ -20,144 +21,299 @@ Definition SymbolicTerm_to_ExprTerm
         end ) t
 .
 
-Definition label {Σ : StaticModel} :=
-    string
-.
 
 
-Definition ContextTemplate
-    {Σ : StaticModel}
+Fixpoint to_transform_sym
+    {A A' B : Type}
+    (f : A -> A')
+    (t : @TermOver' A B)
+    :
+    @TermOver' A' B
 :=
-    forall (br:BasicResolver) (r:Resolver),
-    TermOver operand_type ->
-    TermOver operand_type
+    match t with
+    | t_over o => t_over o
+    | t_term s l => t_term (f s) ((to_transform_sym f) <$>l)
+    end
+.
+
+Inductive StringExpression
+:=
+| se_ground
+    (g : @TermOver' string string)
+| se_variable
+    (x : string)
+| se_apply
+    (s : string)
+    (l : list StringExpression)
 .
 
 
-Notation
-    "( 'context-template' x 'with' h )"
-    :=
-    (fun (_:BasicResolver) (_:Resolver) (h : TermOver operand_type) => x)
+Definition toss_to_option_tosb
+    {Σ : StaticModel}
+    {A : Type}
+    (f : string -> option (builtin_function_symbol+QuerySymbol+builtin_predicate_symbol+builtin_value))
+    (t : @TermOver' A string)
+    :
+    option (@TermOver' A builtin_value)
+:=
+    let f' : string -> option builtin_value := fun x =>
+        match (f x) with
+        | Some (inr bv) => Some bv
+        | _ => None
+        end
+    in
+    TermOver'_option_map f' t
+.
+
+Fixpoint se_to_Expression
+    {Σ : StaticModel}
+    (string2sym : string -> symbol)
+    (string2var : string -> variable)
+    (string2fqpb : string -> option (builtin_function_symbol+QuerySymbol+builtin_predicate_symbol+builtin_value))
+    (se : StringExpression)
+    :
+    option Expression2
+:=
+    match se with
+    | se_ground g =>
+        g' ← toss_to_option_tosb string2fqpb g;
+        Some (e_ground (to_transform_sym string2sym g'))
+    | se_variable x =>
+        Some (e_variable (string2var x))
+    | se_apply s l =>
+        match (string2fqpb s) with
+        | None => None
+        | Some (inl (inl (inl f))) => 
+            let l' := (se_to_Expression string2sym string2var string2fqpb) <$> l in
+            l'' ← list_collect l';
+            Some (e_fun f l'')
+        | Some (inl (inl (inr q))) =>
+            let l' := (se_to_Expression string2sym string2var string2fqpb) <$> l in
+            l'' ← list_collect l';
+            Some (e_query q l'')
+        | Some (inl (inr _)) =>
+            None (* it was a predicate symbol, not a function or query symbol *)
+        | Some (inr b) =>
+            None (* it was a builtin value, not a function or query symbol *)
+        end
+    end
 .
 
 
+Inductive StringSideCondition
+:=
+| ssc_true
+| ssc_false
+| ssc_atom
+    (pred : string)
+    (args : list (StringExpression))
+| ssc_and
+    (left : (StringSideCondition))
+    (right : (StringSideCondition))
+| ssc_or
+    (left : (StringSideCondition))
+    (right : (StringSideCondition))
+.
 
-Record ContextDeclaration {Σ : StaticModel}
+Fixpoint ssc_to_sc
+    {Σ : StaticModel}
+    (string2sym : string -> symbol)
+    (string2var : string -> variable)
+    (string2fqpb : string -> option (builtin_function_symbol+QuerySymbol+builtin_predicate_symbol+builtin_value))
+    (ssc : StringSideCondition)
+    :
+    option SideCondition
+:=
+    match ssc with
+    | ssc_true => Some sc_true
+    | ssc_false => Some sc_false
+    | ssc_atom p args =>
+        p' ← match (string2fqpb p) with
+        | None => None
+        | Some (inl (inl (inl f))) =>
+            None (* function symbol *)
+        | Some (inl (inl (inr q))) =>
+            None (* query symbol *)
+        | Some (inl (inr p)) =>
+            Some p (* predicate symbol *)
+        | Some (inr b) =>
+            None (* builtin value *)
+        end;
+        args' ← list_collect ((se_to_Expression string2sym string2var string2fqpb) <$> args);
+        Some (sc_atom p' args')
+    | ssc_and l r =>
+        left' ← ssc_to_sc string2sym string2var string2fqpb l;
+        right' ← ssc_to_sc string2sym string2var string2fqpb r;
+        Some (sc_and left' right')
+    | ssc_or l r =>
+        left' ← ssc_to_sc string2sym string2var string2fqpb l;
+        right' ← ssc_to_sc string2sym string2var string2fqpb r;
+        Some (sc_or left' right')
+    end
+.
+
+Definition tosse_to_option_tose
+    {Σ : StaticModel}
+    (string2sym : string -> symbol)
+    (string2var : string -> variable)
+    (string2fqpb : string -> option (builtin_function_symbol+QuerySymbol+builtin_predicate_symbol+builtin_value))
+    (t : @TermOver' string StringExpression)
+    :
+    option (TermOver Expression2)
+:=
+    t' ← TermOver'_option_map (se_to_Expression string2sym string2var string2fqpb) t;
+    let t'' := to_transform_sym string2sym t' in
+    Some t''
+.
+
+Variant StringBuiltinOrVar :=
+| sbov_builtin (b : string)
+| sbov_var (x : string)
+.
+
+Definition sbov_to_option_bov
+    {Σ : StaticModel}
+    (string2var : string -> variable)
+    (string2fqpb : string -> option (builtin_function_symbol+QuerySymbol+builtin_predicate_symbol+builtin_value))
+    (sbov : StringBuiltinOrVar)
+    :
+    option BuiltinOrVar
+:=
+    match sbov with
+    | sbov_var x => Some (bov_variable (string2var x))
+    | sbov_builtin b =>
+        b' ← match (string2fqpb b) with
+        | None => None
+        | Some (inl (inl (inl f))) =>
+            None (* function symbol *)
+        | Some (inl (inl (inr q))) =>
+            None (* query symbol *)
+        | Some (inl (inr p)) =>
+            None (* predicate symbol *)
+        | Some (inr b0) =>
+            Some b0 (* builtin value *)
+        end;
+        Some (bov_builtin b')
+    end
+.
+
+Record StringRewritingRule
+    (Act : Set)
+:= mkStringRewritingRule
+{
+    sr_from : @TermOver' string StringBuiltinOrVar ;
+    sr_to : @TermOver' string StringExpression ;
+    sr_scs : StringSideCondition ;
+    sr_act : Act ;
+}.
+
+Definition transl_string_pattern
+    {Σ : StaticModel}
+    (Act : Set)
+    (string2sym : string -> symbol)
+    (string2var : string -> variable)
+    (string2fqpb : string -> option (builtin_function_symbol+QuerySymbol+builtin_predicate_symbol+builtin_value))
+    (p : @TermOver' string StringBuiltinOrVar)
+    :
+    option (TermOver BuiltinOrVar)
+:=
+    let p' := TermOver'_option_map (sbov_to_option_bov string2var string2fqpb) p in
+    p'' ← p';
+    Some (to_transform_sym string2sym p'')
+.
+
+Definition srr_to_rr
+    {Σ : StaticModel}
+    (Act : Set)
+    (string2sym : string -> symbol)
+    (string2var : string -> variable)
+    (string2fqpb : string -> option (builtin_function_symbol+QuerySymbol+builtin_predicate_symbol+builtin_value))
+    (srr : StringRewritingRule Act)
+    :
+    option (RewritingRule2 Act)
+:=
+    match srr with
+    | mkStringRewritingRule _ from to scs act =>
+        from' ← transl_string_pattern Act string2sym string2var string2fqpb from;
+        to' ← tosse_to_option_tose string2sym string2var string2fqpb to;
+        scs' ← ssc_to_sc string2sym string2var string2fqpb scs;
+        Some ({|
+            r_from := from';
+            r_to := to';
+            r_scs := scs';
+            r_act := act;
+        |})
+    end
+.
+
+
+Definition sSymbolicTerm_to_ExprTerm
+    (t : @TermOver' string StringBuiltinOrVar)
+    : @TermOver' string StringExpression
+:=
+    TermOver'_map (fun x:StringBuiltinOrVar =>
+        match x with
+        | sbov_builtin b => se_ground (t_over b)
+        | sbov_var x => se_variable x
+        end ) t
+.
+
+
+Definition ContextTemplate := @TermOver' string StringBuiltinOrVar -> @TermOver' string StringBuiltinOrVar.
+
+Record ContextDeclaration
 := mkContextDeclaration {
-    cd_label : label ;
-    cd_sym : symbol ;
+    cd_label : string ;
+    cd_sym : string ;
     cd_arity : nat ;
     cd_position : nat ;
     cd_positions_to_wait_for : list nat ;
-    cd_isValue : Expression2 -> SideCondition ;
-    cd_isValue_neg : forall e, NegableSideCondition (cd_isValue e) ;
+    cd_isValue : StringExpression -> StringSideCondition ;
     cd_cseq_context : ContextTemplate;
 }.
 
-Record StrictnessDeclaration {Σ : StaticModel}
+Record StrictnessDeclaration
 := mkStrictnessDeclaration {
-    sd_sym : symbol ;
+    sd_sym : string ;
     sd_arity : nat ;
     sd_positions : list nat ;
-    sd_isValue : Expression2 -> SideCondition ;
-    sd_isValue_neg : forall e, NegableSideCondition (sd_isValue e) ;
+    sd_isValue : StringExpression -> StringSideCondition ;
     sd_cseq_context : ContextTemplate ;
 }.
 
-
-Notation
-    "( 'symbol' s 'of' 'arity' a 'strict' 'in' l 'with-result' r 'by-template' t )"
-    :=
-    (
-        (
-            {|
-                sd_sym := s ;
-                sd_arity := a ;
-                sd_positions := l ;
-                sd_isValue := r ;
-                sd_isValue_neg := _;
-                sd_cseq_context := t ;
-            |}
-        )
-    )
-.
-
-Class Defaults {Σ : StaticModel} := {
+Class Defaults := mkDefaults {
     default_cseq_name : string ;
     default_empty_cseq_name : string ;
     default_context_template : ContextTemplate ;
-    default_isValue : Expression2 -> SideCondition ;
-    default_isValue_neg : forall e, NegableSideCondition (default_isValue e) ;
+    default_isValue : StringExpression -> StringSideCondition ;
 }.
 
-Notation
-    "( 'symbol' s 'of' 'arity' a 'strict' 'in' l )"
-:=
-    (
-        (
-            {|
-                sd_sym := s ;
-                sd_arity := a ;
-                sd_positions := l ;
-                sd_isValue := default_isValue ;
-                sd_isValue_neg := default_isValue_neg ;
-                sd_cseq_context := default_context_template ;
-            |}
-        )
-    )
-.
-
 Definition strictness_to_contexts
-    {Σ : StaticModel}
-    (sym_to_str : symbol -> string)
-    (str_to_sym : string -> symbol)
-    (str_to_label : string -> label)
     (sd : StrictnessDeclaration)
     : list ContextDeclaration
 :=
     imap (fun idx position => {|
-            cd_label := (str_to_label (sym_to_str (sd_sym sd) +:+ ("-" +:+ (pretty position)))) ;
+            cd_label := (((sd_sym sd) +:+ ("-" +:+ (pretty position)))) ;
             cd_sym := sd_sym sd ;
             cd_arity := sd_arity sd ;
             cd_position := position ;
             cd_positions_to_wait_for := (firstn idx (sd_positions sd));
             cd_isValue := sd_isValue sd ;
-            cd_isValue_neg := sd_isValue_neg sd ;
-            cd_cseq_context := @sd_cseq_context Σ sd ;
+            cd_cseq_context := sd_cseq_context sd ;
         |})
         (sd_positions sd)
 .
 
-Record RuleDeclaration {Σ : StaticModel} (Act : Set)
+Record RuleDeclaration (Act : Set)
 := mkRuleDeclaration {
-    rd_label : label ;
-    rd_rule : RewritingRule2 Act ;
+    rd_label : string ;
+    rd_rule : StringRewritingRule Act ;
 }.
 
-Arguments mkRuleDeclaration {Σ} {Act} rd_label rd_rule.
-Arguments rd_label {Σ} {Act}%_type_scope r.
-Arguments rd_rule {Σ} {Act}%_type_scope r.
-
-Inductive Declaration {Σ : StaticModel} {Act : Set} :=
-| decl_rule (r : @RuleDeclaration Σ Act)
+Inductive Declaration (Act : Set) :=
+| decl_rule (r : RuleDeclaration Act)
 | decl_ctx (c : ContextDeclaration)
 | decl_strict (s : StrictnessDeclaration)
-.
-
-(*Coercion decl_rule : RuleDeclaration >-> Declaration.*)
-
-Notation "'rule' '[' n ']:' l '~>{' a '}' r"
-    := ((mkRuleDeclaration
-        n (rule (l) ~>{ (a) } (r) requires (sc_true))
-    ))
-    (at level 200)
-.
-
-Notation "'rule' '[' n ']:' l '~>{' a '}' r 'where' s"
-    := ((mkRuleDeclaration
-        n (rule (l) ~>{a} (r) requires s)
-    ))
-    (at level 200)
 .
 
 Definition argument_name
@@ -168,40 +324,59 @@ Definition argument_name
 .
 
 Definition argument_sequence
-    {Σ : StaticModel}
-    (to_var : string -> variable)
     (arity : nat)
-    : list variable
+    : list string
 :=
-    to_var <$> (argument_name <$> (seq 0 arity))
+    (argument_name <$> (seq 0 arity))
 .
 
-Record State {Σ : StaticModel} {Act : Set}
+Record State (Act : Set)
 := mkState {
-    st_rules : gmap label (RewritingRule2 Act) ;
-    st_log : string ;
+    st_rules : (gmap string (StringRewritingRule Act)) ;
 }.
 
-Arguments mkState {Σ} {Act} st_rules st_log%_string_scope.
-
 Definition process_rule_declaration
-    {Σ : StaticModel}
     {Act : Set}
-    (s : State)
+    (s : State Act)
     (r : RuleDeclaration Act)
-    : State
+    : (State Act)+string
 :=
-match (st_rules s) !! (rd_label r) with
+match (st_rules _ s) !! (rd_label _ r) with
 | Some _
-    => (mkState
-        (st_rules s)
-        ((st_log s) +:+ ("Rule with name '" +:+ (rd_label r) ++ "' already present"))%string)
+    => inr
+        ("Rule with name '" +:+ (rd_label _ r) ++ "' already present")%string
 | None
-    => mkState
-        (<[(rd_label r) := (rd_rule r)]>(st_rules s))
-        (st_log s)
+    => inl (mkState Act
+        (<[(rd_label _ r) := (rd_rule _ r)]>(st_rules _ s))
+    )
 end
 .
+
+Fixpoint try_neg_s
+    (sbps_ar : string -> nat)
+    (sbps_neg : string -> option string)
+    (sc : StringSideCondition)
+    : option StringSideCondition
+:= 
+    match sc with
+    | ssc_true => Some ssc_false
+    | ssc_false => Some ssc_true
+    | ssc_and sc1 sc2 =>
+        sc1' ← try_neg_s sbps_ar sbps_neg sc1;
+        sc2' ← try_neg_s sbps_ar sbps_neg sc2;
+        Some (ssc_or sc1' sc2')
+    | ssc_or sc1 sc2 =>
+        sc1' ← try_neg_s sbps_ar sbps_neg sc1;
+        sc2' ← try_neg_s sbps_ar sbps_neg sc2;
+        Some (ssc_and sc1' sc2')
+    | ssc_atom p l =>
+        if decide (length l = sbps_ar p) then 
+            p' ← sbps_neg p;
+            Some (ssc_atom p' l)
+        else None
+    end
+.
+
 
 Section wsm.
     Context
@@ -209,27 +384,23 @@ Section wsm.
         (default_act : Act)
     .
     Context
-        (signature : Signature)
-        (β : Model signature MyUnit)
-        (my_program_info : ProgramInfo)
+        (* (signature : Signature) *)
+        (* (β : Model signature MyUnit) *)
+        (* (my_program_info : ProgramInfo) *)
+        (sbps_ar : string -> nat)
+        (sbps_neg : string -> option string)
     .
 
-    #[local]
-    Instance Σ : StaticModel := default_model signature β my_program_info.
-
-    Definition to_var := fun x:string => x.
-    Definition to_sym := fun x:string => x.
-    
-    Definition REST_SEQ : variable := to_var "$REST_SEQ".
+    Definition REST_SEQ : string := "$REST_SEQ".
 
     Definition cseq {defaults : Defaults} {T : Type}
     :=
-        @t_term _ T (to_sym default_cseq_name)
+        @t_term _ T (default_cseq_name)
     .
 
     Definition emptyCseq {defaults : Defaults} {T : Type}
     :=
-        @t_term _ T (to_sym default_empty_cseq_name)
+        @t_term _ T (default_empty_cseq_name)
     .
 
     Definition freezer
@@ -237,100 +408,104 @@ Section wsm.
         (sym : string)
         (position : nat)
     :=
-        @t_term _ T (to_sym ("freezer_" +:+ sym +:+ "_" +:+ (pretty position)))
+        @t_term _ T (("freezer_" +:+ sym +:+ "_" +:+ (pretty position)))
     .
 
     Definition heating_rule_seq
         {defaults : Defaults}
-        (lbl : label)
-        (freezerLbl : label)
-        (sym : symbol)
+        (lbl : string)
+        (freezerLbl : string)
+        (sym : string)
         (arity : nat)
         (positions_to_wait_for : list nat)
         (position : nat)
-        (isValue : Expression2 -> SideCondition)
-        (isValue_neg : forall e, NegableSideCondition (isValue e))
+        (isValue : StringExpression -> StringSideCondition)
         (cseq_context : ContextTemplate)
-        : RuleDeclaration Act
+        : (RuleDeclaration Act)+string
     :=
-        let vars : list variable
-            := argument_sequence to_var arity in
-        let lhs_vars : list (TermOver BuiltinOrVar)
-            := (t_over <$> (bov_variable <$> vars)) in
-        let rhs_vars : list (TermOver Expression2)
-            := (t_over <$> (e_variable <$> vars)) in
-        let selected_var : variable
-            := to_var (argument_name position) in
-        let lhs_selected_var : (TermOver BuiltinOrVar)
-            := t_over (bov_variable selected_var) in
-        let force_cseq_context
-            := ((fun _:TagLHS => cseq_context _ _) mkTagLHS) in
-        (* all operands on the left are already evaluated *)
-        let side_condition : SideCondition
-            := foldr  sc_and (sc_true) (isValue <$> ((e_variable <$> (to_var <$> (argument_name <$> positions_to_wait_for))) )) in
-        rule [lbl]:
-            cseq_context _ _ (cseq ([
-                (t_term sym lhs_vars);
-                (t_over (bov_variable REST_SEQ))
-            ])%list)
-         ~>{default_act} SymbolicTerm_to_ExprTerm ((force_cseq_context (cseq ([
-                lhs_selected_var;
-                cseq ([
-                    (freezer freezerLbl position (delete position lhs_vars));
-                    (t_over (bov_variable REST_SEQ))
-                ])%list
-            ])%list)))
-            where (sc_and (nsc_negate (isValue (e_variable selected_var))) side_condition)
+        let vars : list string
+            := argument_sequence arity in
+        let lhs_vars : list (@TermOver' string StringBuiltinOrVar)
+            := (map t_over (map sbov_var vars)) in
+        let rhs_vars : list (@TermOver' string StringExpression)
+            := (map t_over (map se_variable vars)) in
+        let selected_var : string
+            := (argument_name position) in
+        match try_neg_s sbps_ar sbps_neg (isValue (se_variable selected_var)) with
+        | None => inr "Cannot negate given isValue condition"
+        | Some is_value_neg => inl (
+            let lhs_selected_var : (@TermOver' string StringBuiltinOrVar)
+                := t_over (sbov_var selected_var) in
+            (* all operands on the left are already evaluated *)
+            let side_condition : StringSideCondition
+                := foldr  ssc_and (ssc_true) (isValue <$> ((se_variable <$> ((argument_name <$> positions_to_wait_for))) )) in
+            (mkRuleDeclaration _ lbl {|
+                sr_from := (cseq_context (cseq ([
+                    (t_term sym lhs_vars);
+                    (t_over (sbov_var REST_SEQ))
+                ])%list));
+                sr_to := (sSymbolicTerm_to_ExprTerm (cseq ([
+                    lhs_selected_var;
+                    cseq ([
+                        (freezer freezerLbl position (delete position lhs_vars));
+                        (t_over (sbov_var REST_SEQ))
+                    ])%list
+                ])));
+                sr_scs := (ssc_and (is_value_neg) side_condition) ;
+                sr_act := default_act ;
+            |})
+            )
+        end
     .
 
 
     Definition cooling_rule
         {defaults : Defaults}
-        (lbl : label)
-        (freezerLbl : label)
-        (sym : symbol)
+        (lbl : string)
+        (freezerLbl : string)
+        (sym : string)
         (arity : nat)
         (position : nat)
-        (isValue : Expression2 -> SideCondition)
+        (isValue : StringExpression -> StringSideCondition)
         (cseq_context : ContextTemplate)
         : RuleDeclaration Act
     :=
-        let vars : list variable
-            := argument_sequence to_var arity in
-        let lhs_vars : list (TermOver BuiltinOrVar)
-            := (t_over <$> (bov_variable <$> vars)) in
-        let rhs_vars : list (TermOver Expression2)
-            := (t_over <$> (e_variable <$> vars)) in
-        let selected_var : variable
-            := to_var (argument_name position) in
-        let lhs_selected_var : (TermOver BuiltinOrVar)
-            := t_over (bov_variable selected_var) in
-        let force_cseq_context
-            := ((fun _:TagLHS => cseq_context _ _) mkTagLHS) in
-        rule [lbl]:
-            cseq_context _ _ (cseq (
+        let vars : list string
+            := argument_sequence arity in
+        let lhs_vars : list (@TermOver' string StringBuiltinOrVar)
+            := (map t_over (map sbov_var vars)) in
+        let rhs_vars : list (@TermOver' string StringExpression)
+            := (map t_over (map se_variable vars)) in
+        let selected_var : string
+            := (argument_name position) in
+        let lhs_selected_var : (@TermOver' string StringBuiltinOrVar)
+            := t_over (sbov_var selected_var) in
+        (mkRuleDeclaration _ lbl {|
+            sr_from := (cseq_context (cseq (
                 ([
                 lhs_selected_var;
                 cseq ([
                     (freezer freezerLbl position (delete position lhs_vars));
-                    (t_over (bov_variable REST_SEQ))
+                    (t_over (sbov_var REST_SEQ))
                 ])%list
             ])%list
-           ))
-         ~>{default_act} SymbolicTerm_to_ExprTerm ((force_cseq_context (cseq [
+           )));
+            sr_to := (sSymbolicTerm_to_ExprTerm (((cseq [
                 (t_term sym lhs_vars);
-                (t_over (bov_variable REST_SEQ))
-            ])%list))
-            where (isValue (e_variable selected_var))
+                (t_over (sbov_var REST_SEQ))
+            ])%list)));
+            sr_act := default_act;
+            sr_scs := (isValue (se_variable selected_var));
+        |})
     .
 
     Definition process_context_declaration
         {defaults : Defaults}
-        (s : State)
+        (s : State Act)
         (c : ContextDeclaration)
-        : State
+        : (State Act)+string
     := 
-        let hr : RuleDeclaration Act
+        let hr' : (RuleDeclaration Act)+string
             := heating_rule_seq
                     ((cd_label c) +:+ "-heat")
                     (cd_label c)
@@ -339,77 +514,81 @@ Section wsm.
                     (cd_positions_to_wait_for c)
                     (cd_position c)
                     (cd_isValue c)
-                    (cd_isValue_neg c)
-                    (@cd_cseq_context Σ c)
+                    (cd_cseq_context c)
             in
-        let cr : RuleDeclaration Act
-            := cooling_rule
-                    ((cd_label c) +:+ "-cool")
-                    (cd_label c)
-                    (cd_sym c)
-                    (cd_arity c)
-                    (cd_position c)
-                    (cd_isValue c)
-                    (@cd_cseq_context Σ c)
-            in
-        
-        process_rule_declaration
-            (process_rule_declaration s hr)
-            cr
+        match hr' with
+        | inl hr => (
+            let cr : RuleDeclaration Act
+                := cooling_rule
+                        ((cd_label c) +:+ "-cool")
+                        (cd_label c)
+                        (cd_sym c)
+                        (cd_arity c)
+                        (cd_position c)
+                        (cd_isValue c)
+                        (cd_cseq_context c)
+                in
+            
+            match (process_rule_declaration s hr) with
+            | inl s' =>
+                process_rule_declaration
+                    s'
+                    cr
+            | inr err_s =>
+                inr ("Cannot process declaration: " +:+ err_s)
+            end
+        )
+        | (inr err_s) =>
+            inr ("Invalid 'context' declaration: " +:+ err_s)
+        end
     .
 
     Definition process_strictness_declaration
         {defaults : Defaults}
-        (s : State)
+        (s : State Act)
         (c : StrictnessDeclaration)
-        : State
+        : (State Act)+string
     :=
         foldr
-            (fun a b => process_context_declaration b a)
-            s
-            (strictness_to_contexts id id id c)
+            (fun a b' => match b' with inr s => inr s | inl b => process_context_declaration b a end)
+            (inl s)
+            (strictness_to_contexts c)
     .
 
     Definition initialState
-        {Σ : StaticModel}
-        : @State Σ Act
+        : State Act
     := {|
         st_rules := ∅ ;
-        st_log := "";
     |}.
 
 
 
     Definition process_declaration
         {defaults : Defaults}
-        (s : State)
-        (d : Declaration)
-        : State
+        (s : State Act)
+        (d : Declaration Act)
+        : (State Act)+string
     :=
     match d with
-    | decl_rule rd => process_rule_declaration s rd
-    | decl_ctx cd => process_context_declaration s cd
-    | decl_strict sd => process_strictness_declaration s sd
+    | decl_rule _ rd => process_rule_declaration s rd
+    | decl_ctx _ cd => process_context_declaration s cd
+    | decl_strict _ sd => process_strictness_declaration s sd
     end.
 
     Definition process_declarations
         {defaults : Defaults}
-        (ld : list Declaration)
-        : State
+        (ld : list (Declaration Act))
+        : (State Act)+string
     :=
-        fold_left process_declaration ld initialState
+        fold_left (fun s' d => match s' with inl s => process_declaration s d | inr s => inr s end) ld (inl initialState)
     .
 
     Definition to_theory
-        {Σ : StaticModel}
-        (s : State)
-        : (list (RewritingRule2 Act))*(list string)
+        (s : State Act)
+        : (list (StringRewritingRule Act))*(list string)
     :=
-        let l := (map_to_list (st_rules s)) in
+        let l := (map_to_list (st_rules _ s)) in
         (l.*2,l.*1)
     .
 
 End wsm.
-
-
-
