coq-minuska/theories/signature_morphism.v
@@ -19,6 +19,9 @@ Arguments builtin_predicate_interp {symbol} {symbols signature}
 Record SignatureMorphism (s1 s2 : Signature) := {
     function_symbol_morphism : (builtin_function_symbol s1) -> (builtin_function_symbol s2) ;
     predicate_symbol_morphism : (builtin_predicate_symbol s1) -> (builtin_predicate_symbol s2) ;
+    sm_pred_ar : forall p, bps_ar (predicate_symbol_morphism p) = bps_ar p ;
+    sm_pred_neg : forall p,
+      bps_neg (predicate_symbol_morphism p) = predicate_symbol_morphism <$> (bps_neg p) ;
 }.
 
 Arguments function_symbol_morphism {s1 s2} s _.
