languages/decrement-builtin/def.m
@@ -6,7 +6,7 @@
 @rule [init]: builtin.init[] => cfg[program.ast()] where @true ;
 
 @rule [decrement]:
-	cfg[X] => cfg[z.minus(X, [(@builtin-int 1)])] where @true
+	cfg[X] => cfg[z.minus(X, [(@builtin:int("1"))])] where @true
     ;
 
 
